$$
\begin{aligned}
    &3.\lim_{x\to 0}\frac{(1+x)^{\frac 2x}-e^2[1-ln(1+x)]}{x}\\
    &=\lim_{x\to 0}\frac{(1+x)^{\frac 2x}-e^2+e^2ln(1+x)}{x}\\
    &=\lim_{x\to 0}\frac{(1+x)^{\frac 2x}-e^2}{x}+\lim_{x\to 0}\frac{e^2ln(1+x)}{x}(能拆是因为极限都存在)\\
    &=\lim_{x\to 0}\frac{e^{\frac 2xln(1+x)}-e^2}{x}+e^2\\
    &=\lim_{x\to 0}\frac{e^2(e^{\frac 2xln(1+x)-2}-1)}{x}+e^2\\
    &=\lim_{x\to 0}\frac{e^2(\frac 2xln(1+x)-2)}{x}+e^2\\
    &=\lim_{x\to 0}\frac{e^2(2ln(1+x)-2x)}{x^2}+e^2\\
    &=2e^2\lim_{x\to 0}\frac{ln(1+x)-x}{x^2}+e^2\\
    &=2e^2\lim_{x\to 0}\frac{x-\frac{x^2}{2}-x}{x^2}+e^2\\
    &=2e^2\lim_{x\to 0}\frac{-\frac{x^2}{2}}{x^2}+e^2\\
    &=2e^2*-\frac 12+e^2\\
    &=0\\
    &5.\lim_{x\to 0}\frac{\sqrt{1-x^2}\sin^2x - \tan^2 x}{x^2[ln(1+x)^2]}\\
    &=\lim_{x\to 0}\frac{\sqrt{1-x^2}\sin^2x - \tan^2 x}{x^4}\\
    &6.\lim_{x\to 0}\frac{(3+2\tan x)^x -3^x}{3\sin^2 x + x^2cos \frac 1x}\\
    &=\lim_{x\to 0}\frac{3^x(1+\frac{2}{3}\tan x)^x -1}{3x^2}(x^2\cos \frac {1}{x}是比3\sin^2 x高阶的无穷小,高阶无穷小+低阶无穷小=低阶无穷小)\\
    &=\lim_{x\to 0}3^x*\lim_{x\to 0}\frac{(1+\frac{2}{3}\tan x)^x -1}{3x^2}\\
    &=\lim_{x\to 0}\frac{e^{xln(1+\frac{2}{3}\tan x)} -1}{3x^2}\\
    &=\lim_{x\to 0}\frac{xln(1+\frac{2}{3}\tan x)}{3x^2}\\
    &=\lim_{x\to 0}\frac{\frac{2}{3}\tan x}{3x^2}\\
    &=\lim_{x\to 0}\frac{\frac{2}{3} x}{3x^2}\\
    &=\frac 29\\
    &7.\lim_{x\to 2}\frac{\sqrt{5x-1}-\sqrt{2x+5}}{x^2-4}\\
    &=\lim_{x\to 2}\frac{\sqrt{5x-1}-\sqrt{2x+5}}{x^2-4}(分子有理化)\\
    &=\lim_{x\to 2}\frac{3x-6}{(x^2-4)(\sqrt{5x-1}+\sqrt{2x+5)}}\\
    &=\lim_{x\to 2}\frac{3(x-2)}{(x-2)(x+2)(\sqrt{5x-1}+\sqrt{2x+5)}}\\
    &=\lim_{x\to 2}\frac{3}{(x+2)(\sqrt{5x-1}+\sqrt{2x+5)}}\\
    &=\frac 18 (连续函数的极限值等于函数值)\\


\end{aligned}
$$      